examples/new_stack/NewStack1.v
@@ -20,10 +20,6 @@ Section PROOF.
   Context `{Σ: GRA.t}.
   Context `{@GRA.inG memRA Σ}.
 
-  Definition new_spec: fspec := fspec_trivial.
-  Definition pop_spec: fspec := fspec_trivial.
-  Definition push_spec: fspec := fspec_trivial.
-
   Notation pget := (p0 <- trigger PGet;; `p0: (gmap mblock (list Z)) <- p0↓ǃ;; Ret p0) (only parsing).
   Notation pput p0 := (trigger (PPut (p0: (gmap mblock (list Z)))↑)) (only parsing).
 
@@ -65,7 +61,7 @@ Section PROOF.
       match stk0 with
       | x :: stk1 =>
         stk_mgr2 <- pget;; pput (<[handle:=stk1]> stk_mgr2);;;
-        trigger (kCall false false "debug" ([Vint 0; Vint x]↑));;;
+        trigger (kCall unknown "debug" ([Vint 0; Vint x]↑));;;
         Ret (Vint x)
       | _ =>
         stk_mgr2 <- pget;; pput (<[handle:=[]]> stk_mgr2);;;
@@ -87,14 +83,14 @@ Section PROOF.
       let stk_mgr1 := delete handle stk_mgr0 in pput stk_mgr1;;;
       APCK;;;
       stk_mgr2 <- pget;; pput (<[handle:=(x :: stk0)]> stk_mgr2);;;
-      trigger (kCall false false "debug" ([Vint 1; Vint x]↑));;;
+      trigger (kCall unknown "debug" ([Vint 1; Vint x]↑));;;
       Ret Vundef
   .
 
   Definition StackSbtb: list (gname * kspecbody) :=
-    [("new", mk_kspecbody new_spec (cfun new_body) (cfun new_body));
-    ("pop", mk_kspecbody pop_spec (cfun pop_body) (cfun pop_body));
-    ("push",   mk_kspecbody push_spec (cfun push_body) (cfun push_body))
+    [("new", ksb_trivial (cfun new_body));
+    ("pop", ksb_trivial (cfun pop_body));
+    ("push", ksb_trivial (cfun push_body))
     ].
 
   Definition StackStb: list (gname * fspec).
@@ -116,20 +112,18 @@ Section PROOF.
     KModSem.initial_st := (gmap_empty: gmap mblock (list Z))↑;
   |}
   .
-
-  Definition SStackSem: SModSem.t := (KModSem.to_tgt) KStackSem.
-
+  Definition SStackSem: SModSem.t := KStackSem.
   Definition StackSem (stb: list (string * fspec)): ModSem.t :=
     (SModSem.to_tgt stb) SStackSem.
+
+
 
   Definition KStack: KMod.t := {|
     KMod.get_modsem := fun _ => KStackSem;
     KMod.sk := Sk.unit;
   |}
   .
-
-  Definition SStack: SMod.t := (KMod.to_tgt) KStack.
-
+  Definition SStack: SMod.t := KStack.
   Definition Stack (stb: Sk.t -> list (string * fspec)): Mod.t :=
     SMod.to_tgt stb SStack.
 
