mem/MemOpen.v
@@ -108,19 +108,17 @@ Section PROOF.
     KModSem.initial_st := (Sk.load_mem sk)↑;
   |}
   .
-
-  Definition SMemSem: Sk.t -> SModSem.t := (KModSem.to_tgt) ∘ KMemSem.
-
+  Definition SMemSem: Sk.t -> SModSem.t := KMemSem.
   Definition MemSem (stb: list (gname * fspec)): Sk.t -> ModSem.t := (SModSem.to_tgt stb) ∘ SMemSem.
+
+
 
   Definition KMem: KMod.t := {|
     KMod.get_modsem := KMemSem;
     KMod.sk := Sk.unit;
   |}
   .
-
-  Definition SMem: SMod.t := (KMod.to_tgt) KMem.
-
+  Definition SMem: SMod.t := KMem.
   Definition Mem (stb: Sk.t -> list (gname * fspec)): Mod.t := SMod.to_tgt stb SMem.
 
 End PROOF.
